code/experimental/rsa/Hacl.RSAPSS.fst
@@ -13,8 +13,7 @@ module Buffer = Spec.Lib.IntBuf
 
 val rsa_pss_sign:
     #sLen:size_nat -> #msgLen:size_nat -> #nLen:size_nat ->
-    pow2_i:size_t{9 * (1 + nLen) + 4 * v pow2_i < max_size_t /\ (1 + nLen) < v pow2_i} ->
-    iLen:size_t{v iLen < v pow2_i / 2 /\ v iLen + (1 + nLen) = v pow2_i} ->
+    pow2_i:size_t{6 * nLen + 4 * v pow2_i < max_size_t /\ nLen <= v pow2_i /\ nLen + 1 < 2 * v pow2_i} ->
     modBits:size_t{0 < v modBits /\ nLen = v (bits_to_bn modBits)} ->
     eBits:size_t{0 < v eBits /\ v eBits <= v modBits} ->
     dBits:size_t{0 < v dBits /\ v dBits <= v modBits} ->
@@ -28,15 +27,14 @@ val rsa_pss_sign:
 	              disjoint msg salt /\ disjoint msg sgnt /\ disjoint sgnt salt))
     (ensures (fun h0 _ h1 -> preserves_live h0 h1 /\ modifies1 sgnt h0 h1))
 
-let rsa_pss_sign #sLen #msgLen #nLen pow2_i iLen modBits eBits dBits pLen qLen skey rBlind ssLen salt mmsgLen msg sgnt =
+let rsa_pss_sign #sLen #msgLen #nLen pow2_i modBits eBits dBits pLen qLen skey rBlind ssLen salt mmsgLen msg sgnt =
     //push_frame();
-    Hacl.Impl.RSA.rsa_sign #sLen #msgLen #nLen pow2_i iLen modBits eBits dBits pLen qLen skey rBlind ssLen salt mmsgLen msg sgnt
+    Hacl.Impl.RSA.rsa_sign #sLen #msgLen #nLen pow2_i modBits eBits dBits pLen qLen skey rBlind ssLen salt mmsgLen msg sgnt
     //pop_frame()
 
 val rsa_pss_verify:
     #sLen:size_nat -> #msgLen:size_nat -> #nLen:size_nat ->
-    pow2_i:size_t{9 * (1 + nLen) + 4 * v pow2_i < max_size_t /\ (1 + nLen) < v pow2_i} ->
-    iLen:size_t{v iLen < v pow2_i / 2 /\ v iLen + (1 + nLen) = v pow2_i} ->
+    pow2_i:size_t{6 * nLen + 4 * v pow2_i < max_size_t /\ nLen <= v pow2_i /\ nLen + 1 < 2 * v pow2_i} ->
     modBits:size_t{0 < v modBits /\ nLen = v (bits_to_bn modBits)} ->
     eBits:size_t{0 < v eBits /\ v eBits <= v modBits /\ nLen + v (bits_to_bn eBits) < max_size_t} ->
     pkey:lbignum (nLen + v (bits_to_bn eBits)) ->
@@ -46,8 +44,8 @@ val rsa_pss_verify:
     (requires (fun h -> live h msg /\ live h sgnt /\ live h pkey /\ disjoint msg sgnt))
     (ensures (fun h0 _ h1 -> preserves_live h0 h1 /\ modifies0 h0 h1))
 
-let rsa_pss_verify #sLen #msgLen #nLen pow2_i iLen modBits eBits pkey ssLen sgnt mmsgLen msg =
+let rsa_pss_verify #sLen #msgLen #nLen pow2_i modBits eBits pkey ssLen sgnt mmsgLen msg =
     //push_frame();
-    let res = Hacl.Impl.RSA.rsa_verify #sLen #msgLen pow2_i iLen modBits eBits pkey ssLen sgnt mmsgLen msg in
+    let res = Hacl.Impl.RSA.rsa_verify #sLen #msgLen pow2_i modBits eBits pkey ssLen sgnt mmsgLen msg in
     //pop_frame();
     res
