code/experimental/rsa/Hacl.Impl.Multiplication.fst
@@ -86,44 +86,37 @@ type sign =
      | Negative : sign
 
 val abs:
-    #aLen:size_nat -> #bLen:size_nat ->
-    aaLen:size_t{v aaLen == aLen} -> a:lbignum aLen ->
-    bbLen:size_t{v bbLen == bLen /\ bLen <= aLen} -> b:lbignum bLen ->
+    #aLen:size_nat -> aaLen:size_t{v aaLen == aLen} ->
+    a:lbignum aLen -> b:lbignum aLen ->
     res:lbignum aLen -> Stack sign
     (requires (fun h -> live h a /\ live h b /\ live h res /\ disjoint a b))
     (ensures  (fun h0 _ h1 -> preserves_live h0 h1 /\ modifies1 res h0 h1))
     [@"c_inline"]
-let abs #aLen #bLen aaLen a bbLen b res =
-    if (bn_is_less aaLen a bbLen b) //a < b
+let abs #aLen aaLen a b res =
+    if (bn_is_less aaLen a aaLen b) //a < b
     then begin
-      let a' = Buffer.sub #uint64 #aLen #bLen a (size 0) bbLen in
-      let res' = Buffer.sub #uint64 #aLen #bLen res (size 0) bbLen in
-      bn_sub bbLen b bbLen a' res';
+      bn_sub aaLen b aaLen a res;
       Negative end
     else begin
-      bn_sub aaLen a bbLen b res;
+      bn_sub aaLen a aaLen b res;
       Positive end
 
 val add_sign:
-    #a0Len:size_nat -> #a1Len:size_nat -> #resLen:size_nat ->
-    aa0Len:size_t{v aa0Len == a0Len} ->
-    aa1Len:size_t{v aa1Len == a1Len /\ a1Len <= a0Len} ->
-    rresLen:size_t{v rresLen == resLen /\ resLen = a0Len + a0Len + 1 /\ resLen < max_size_t} ->
-    c0:lbignum (a0Len + a0Len) -> c1:lbignum (a1Len + a1Len) -> c2:lbignum (a0Len + a0Len) ->
-    a0:lbignum a0Len -> a1:lbignum a1Len -> a2:lbignum a0Len ->
-    b0:lbignum a0Len -> b1:lbignum a1Len -> b2:lbignum a0Len ->
+    #a0Len:size_nat -> aa0Len:size_t{v aa0Len == a0Len /\ a0Len + a0Len + 1 < max_size_t} ->
+    c0:lbignum (a0Len + a0Len) -> c1:lbignum (a0Len + a0Len) -> c2:lbignum (a0Len + a0Len) ->
+    a0:lbignum a0Len -> a1:lbignum a0Len -> a2:lbignum a0Len ->
+    b0:lbignum a0Len -> b1:lbignum a0Len -> b2:lbignum a0Len ->
     sa2:sign -> sb2:sign ->
-    res:lbignum (v rresLen) -> Stack unit
+    rresLen:size_t{v rresLen = a0Len + a0Len + 1} -> res:lbignum (v rresLen) -> Stack unit
     (requires (fun h -> live h c0 /\ live h c1 /\ live h c2 /\ 
                       live h a0 /\ live h a1 /\ live h a2 /\
                       live h b0 /\ live h b1 /\ live h b2 /\
 		      live h res /\ disjoint a0 a1 /\ disjoint b0 b1))
     (ensures (fun h0 _ h1 -> preserves_live h0 h1 /\ modifies1 res h0 h1))
     [@"c_inline"]
-let add_sign #a0Len #a1Len #resLen aa0Len aa1Len rresLen c0 c1 c2 a0 a1 a2 b0 b1 b2 sa2 sb2 res =
+let add_sign #a0Len aa0Len c0 c1 c2 a0 a1 a2 b0 b1 b2 sa2 sb2 rresLen res =
     let c0Len = add #SIZE aa0Len aa0Len in
-    let c1Len = add #SIZE aa1Len aa1Len in
-    bn_add_carry c0Len c0 c1Len c1 res;
+    bn_add_carry c0Len c0 c0Len c1 res;
     if ((sa2 = Positive && sb2 = Positive) || (sa2 = Negative && sb2 = Negative))
     then bn_sub rresLen res c0Len c2 res
     else bn_add rresLen res c0Len c2 res
@@ -134,8 +127,7 @@ val karatsuba_:
     aaLen:size_t{v aaLen == aLen /\ aLen + aLen < max_size_t /\ v pow2_i = aLen} ->
     a:lbignum aLen -> b:lbignum aLen -> tmp:lbignum (4 * v pow2_i) ->
     res:lbignum (aLen + aLen) -> Stack unit
-    (requires (fun h -> live h a /\ live h b /\ live h tmp /\ live h res /\ disjoint res tmp
-                   /\ disjoint tmp a /\ disjoint tmp b /\ disjoint res a /\ disjoint res b))
+    (requires (fun h -> live h a /\ live h b /\ live h tmp /\ live h res /\ disjoint res a /\ disjoint res b))
     (ensures  (fun h0 _ h1 -> preserves_live h0 h1 /\ modifies2 res tmp h0 h1))
     #reset-options "--z3rlimit 150 --max_fuel 2"
     [@"c_inline"]
@@ -163,8 +155,8 @@ let rec karatsuba_ #aLen pow2_i aaLen a b tmp res =
 
        let a2 = Buffer.sub #uint64 #(v tmpLen) #(v pow2_i0) tmp (size 0) pow2_i0 in
        let b2 = Buffer.sub #uint64 #(v tmpLen) #(v pow2_i0) tmp pow2_i0 pow2_i0 in
-       let sa2 =  abs #(v pow2_i0) #(v pow2_i0) pow2_i0 a0 pow2_i0 a1 a2 in // a2 = |a0 - a1|
-       let sb2 = abs #(v pow2_i0) #(v pow2_i0) pow2_i0 b0 pow2_i0 b1 b2 in // b2 = |b0 - b1|
+       let sa2 =  abs #(v pow2_i0) pow2_i0 a0 a1 a2 in // a2 = |a0 - a1|
+       let sb2 = abs #(v pow2_i0) pow2_i0 b0 b1 b2 in // b2 = |b0 - b1|
 
        let c2 = Buffer.sub #uint64 #(v tmpLen) #(v pow2_i) tmp pow2_i pow2_i in
        let tmp0 = Buffer.sub #uint64 #(v tmpLen) #(4 * v pow2_i0) tmp (mul #SIZE (size 4) pow2_i0) (mul #SIZE (size 4) pow2_i0) in
@@ -172,17 +164,15 @@ let rec karatsuba_ #aLen pow2_i aaLen a b tmp res =
 
        let tmp1Len = size_incr pow2_i in
        let tmp1 = Buffer.sub #uint64 #(v tmpLen) #(v tmp1Len) tmp (mul #SIZE (size 4) pow2_i0) tmp1Len in
-       add_sign #(v pow2_i0) #(v pow2_i0) #(v tmp1Len) pow2_i0 pow2_i0 tmp1Len c0 c1 c2 a0 a1 a2 b0 b1 b2 sa2 sb2 tmp1; //tmp1 = (c0 + c1) +/- c2
+       add_sign #(v pow2_i0) pow2_i0 c0 c1 c2 a0 a1 a2 b0 b1 b2 sa2 sb2 tmp1Len tmp1; //tmp1 = (c0 + c1) +/- c2
 
        //res = [c0; c1]
        //tmp = [a2; b2; c2; tmp1; _]
-       let res1Len = add #SIZE pow2_i0 (add #SIZE pow2_i0 pow2_i0) in
+       let res1Len = add #SIZE pow2_i0 pow2_i in
        let res1 = Buffer.sub #uint64 #(v resLen) #(v res1Len) res pow2_i0 res1Len in
        bn_add res1Len res1 tmp1Len tmp1 res1
     end); admit()
 
-// aLen + iLen == pow2_i
-// iLen is the number of leading zeroes
 val karatsuba:
     #aLen:size_nat ->
     pow2_i:size_t{2 * aLen + 4 * v pow2_i < max_size_t} ->
@@ -193,15 +183,14 @@ val karatsuba:
     (requires (fun h -> live h a /\ live h b /\ live h st_kara /\
                       disjoint st_kara a /\ disjoint st_kara b))
     (ensures  (fun h0 _ h1 -> preserves_live h0 h1 /\ modifies1 st_kara h0 h1))
+    #reset-options "--z3rlimit 50 --max_fuel 0"
     [@"c_inline"]
 let karatsuba #aLen pow2_i aaLen a b st_kara =
     let stLen = add #SIZE (add #SIZE aaLen aaLen) (mul (size 4) pow2_i) in
     let res = Buffer.sub #uint64 #(v stLen) #(aLen + aLen) st_kara (size 0) (add #SIZE aaLen aaLen) in
     let st_mult = Buffer.sub #uint64 #(v stLen) #(4 * v pow2_i) st_kara (add #SIZE aaLen aaLen) (mul #SIZE (size 4) pow2_i) in
-    if not (pow2_i =. aaLen) 
+    disjoint_sub_lemma1 st_kara a (size 0) (add #SIZE aaLen aaLen); // disjoint res a
+    disjoint_sub_lemma1 st_kara b (size 0) (add #SIZE aaLen aaLen); // disjoint res b
+    (if not (pow2_i =. aaLen) 
     then bn_mul #aLen #aLen aaLen a aaLen b res
-    else karatsuba_ pow2_i aaLen a b st_mult res
-
-    (*if (aaLen <. size 32)
-    then bn_mul #aLen #aLen aaLen a aaLen b res
-    else karatsuba_ pow2_i iLen aaLen a b st_mult res*)
+    else karatsuba_ pow2_i aaLen a b st_mult res); admit()
